[SI] wip but need to redo the new RA

aneris/examples/snapshot_isolation/proof/resources/server_resources.v
@@ -9,24 +9,27 @@ From aneris.algebra Require Import monotone.
 From aneris.aneris_lang Require Import lang resources resources inject.
 From aneris.lib Require Import gen_heap_light.
 From aneris.aneris_lang.lib Require Import
-     list_proof monitor_proof lock_proof map_proof.
+     list_proof lock_proof map_proof.
 From aneris.aneris_lang.lib.serialization Require Import serialization_proof.
-From aneris.examples.snapshot_isolation.specs Require Import user_params.
-From aneris.examples.snapshot_isolation.proof Require Import time events model.
-From aneris.examples.snapshot_isolation.proof.resources Require Import resource_algebras.
+From aneris.examples.snapshot_isolation.proof Require Import model.
+From aneris.examples.snapshot_isolation.proof.resources Require Import
+  resource_algebras.
 
 
+(*----------------------------------------------------------------------------*)
+(** Meta tokens tracking connection between physical data and ghost names.    *)
+(*----------------------------------------------------------------------------*)
 
-(** Meta tokens tracking connection between physical data and ghost names. *)
 Section ConnectedClients.
   Context `{!anerisG Mdl Σ, !IDBG Σ}.
-
   Context (γKnownClients : gname).
 
-  Definition connected_clients (M : gmap socket_address gname) : iProp Σ :=
+  Definition connected_clients
+    (M : gmap socket_address gname) : iProp Σ :=
     own γKnownClients (● (to_agree <$> M : gmap _ _)).
 
-  Definition connected_client_token (sa : socket_address) (γCst : gname) : iProp Σ :=
+  Definition connected_client_token
+    (sa : socket_address) (γCst : gname) : iProp Σ :=
     own γKnownClients (◯ {[ sa := to_agree γCst ]}).
 
   Global Instance session_tokenPersistent sa γ :
@@ -34,7 +37,9 @@ Section ConnectedClients.
   Proof. apply _. Qed.
 
   Lemma session_token_agree sa γ1 γ2 :
-    connected_client_token sa γ1 -∗ connected_client_token sa γ2 -∗ ⌜γ1 = γ2⌝.
+    connected_client_token sa γ1 -∗
+    connected_client_token sa γ2 -∗
+    ⌜γ1 = γ2⌝.
   Proof.
     iIntros "Hγ1 Hγ2".
     iDestruct (own_valid_2 with "Hγ1 Hγ2") as %Hval.
@@ -52,135 +57,304 @@ Section ConnectedClients.
 
 End ConnectedClients.
 
-Section Resources.
+(*----------------------------------------------------------------------------*)
+(** Resources embedding the model of the global memory and snapshots.         *)
+(*----------------------------------------------------------------------------*)
+
+(*---------------------------------------------------------------------------*)
+(** ----------------------- Resources for Snapshots ------------------------ *)
+(*---------------------------------------------------------------------------*)
+Section Snapshot_Resources.
   Context `{!anerisG Mdl Σ, !User_params, !IDBG Σ}.
+  Context (γTrns : gname).
 
-  Context (γGauth γGsnap γT γTss : gname).
+  (** Snapshots related to a transaction identified by a ghost name γt. *)
+  Section Snapshot_at_given_gname.
+    Context (γt : gname).
+    
+    Definition ownSnapFragGname (k : Key) (h : whist) : iProp Σ :=
+      own γt (◯ {[ k := to_max_prefix_list h]}).
 
-  (** ---------------- Global memory ---------------- *)
+    Lemma ownSnapFragGnamePersistent k h:
+      Persistent (ownSnapFragGname k h).
+    Proof. apply _. Qed.
+  
+    Definition global_memUR M : gmapUR Key (max_prefix_listR write_eventO) :=
+      (to_max_prefix_list <$> M :
+        gmapUR Key (max_prefix_listR write_eventO)).
 
-  Definition ownMemSeen (k : Key) (h : list write_event) : iProp Σ :=
-    own γGsnap (◯ {[ k := to_max_prefix_list h]}).
+    Definition ownSnapFragMemGname M : iProp Σ :=
+      own γt (◯ global_memUR M).
 
-  Definition ownMemUser (k : Key) (h : (list write_event)) : iProp Σ :=
-    ghost_map_elem γGauth k (DfracOwn 1%Qp) h ∗
-      ownMemSeen k h.
+    Lemma ownSnapFragMemGnamePersistent M:
+      Persistent (ownSnapFragMemGname M).
+    Proof. apply _. Qed.
+    
+    Definition ownSnapAuthGname (M : global_mem) : iProp Σ :=
+      own γt (● global_memUR M).
 
-  Definition ownMemAuthGlobal
-             (M : gmap Key (list write_event)) :=
-    ghost_map_auth γGauth (1/2)%Qp M.
+    Lemma ownSnapFragGname_lookup M k h :
+      ownSnapAuthGname M ⊢
+      ownSnapFragGname k h -∗
+      ∃ h', ⌜h `prefix_of` h' ∧ M !! k = Some h'⌝.
+    Proof.
+      iIntros "H1 H2".
+      iDestruct (own_valid_2 with "H1 H2")
+        as %[Hv1 Hv2]%auth_both_valid_discrete.
+      rewrite singleton_included_l in Hv1.
+      destruct Hv1 as (y & Hvy & Hv1).
+      rewrite Some_included_total in Hv1.
+      rewrite lookup_fmap in Hvy.
+      destruct (M !! k) eqn:Heq; rewrite Heq in Hvy;
+        simplify_eq /=; [| by inversion Hvy].
+      apply Some_equiv_inj in Hvy.
+      rewrite -Hvy to_max_prefix_list_included in Hv1.
+      destruct Hv1 as (l0 & Hl0).
+      fold_leibniz.
+      iPureIntro; exists l. split; last done.
+      by rewrite Hl0; apply prefix_app_r.
+    Qed.
 
-  Definition ownMemAuthLocal (M : gmap Key (list write_event)) :=
-    ghost_map_auth γGauth (1/2)%Qp M.
+    (* We do not need this lemma actually *)
+    (* Lemma ownSnapFragGname_prefix k h h':
+      ownSnapFragGname k h ⊢ ownSnapFragGname k h' -∗
+        ⌜h `prefix_of` h' ∨ h' `prefix_of` h⌝.
+    Proof.
+      iIntros "Hobs1 Hobs2".
+      iDestruct (own_valid_2 with "Hobs1 Hobs2") as %Hvalid.
+      rewrite auth_frag_op_valid singleton_op singleton_valid
+        in Hvalid.
+      by rewrite to_max_prefix_list_op_valid_L in Hvalid.
+    Qed. *)
 
-  Definition ownMemMono (M : gmap Key (list write_event)) : iProp Σ :=
-    own γGsnap
-        (● (to_max_prefix_list <$> M : gmapUR Key (max_prefix_listR write_eventO))).
+    Lemma get_ownSnapFragGname_prefix M k h hl:
+      M !! k = Some h →
+      hl `prefix_of` h →
+      ownSnapAuthGname M ⊢
+        |==> ownSnapAuthGname M ∗ ownSnapFragGname k hl.
+    Proof.
+      iIntros (HMk h_hl) "?".
+      iApply own_op.
+      iApply own_update; last done.
+      apply auth_update_dfrac_alloc.
+      {
+        apply gmap_core_id=>i x/lookup_singleton_Some[_<-].
+        apply max_prefix_list.mono_list_lb_core_id.
+      }
+      apply (@singleton_included_l _ _ _ (max_prefix_listR write_eventO)).
+      exists (to_max_prefix_list h).
+      split; first by rewrite lookup_fmap HMk.
+      apply Some_included_2.
+      apply (@to_max_prefix_list_included_L write_eventO); last done.
+      apply _.
+    Qed.
+  
+  Lemma get_ownSnapFragGname M k h :
+      M !! k = Some h →
+      ownSnapAuthGname M ⊢ |==> ownSnapAuthGname M ∗ ownSnapFragGname k h.
+  Proof.
+    intro HMk.
+    by iApply get_ownSnapFragGname_prefix.
+  Qed.
+  
+  End Snapshot_at_given_gname.
 
-  Definition ownMemGlobal (M : gmap Key (list write_event)) : iProp Σ :=
-    ownMemAuthGlobal M ∗ ownMemMono M.
+  Section Snapshots.
+    
+    (** A transaction identified by the start time ts and a ghost name γTr. *)
+    Definition ownTrnFrag (t : nat) (γt : gname) : iProp Σ :=
+      own γTrns (◯ {[ t := to_agree γt ]}).
 
-  (** ---------------- Time Snaps ---------------- *)
-  Definition ownTimeStartsAuth (tss : gset nat) : iProp Σ :=
-    own γTss (● tss).
+    Definition ownSnapshotsNamesAuth (S : gmap nat gname) : iProp Σ :=
+      own γTrns (● (to_agree <$> S : gmap _ _)).
 
-  Definition ownTimeStartsSnap (t : nat) : iProp Σ :=
-    own γTss (◯ {[ t ]}).
+    Definition ownSnapFrag γt (t : nat) (k : Key) (h : whist) : iProp Σ :=
+      ownTrnFrag t γt ∗ ownSnapFragGname γt k h .
 
-  (** ---------------- Time ---------------- *)
-  Definition ownTimeGlobal T : iProp Σ :=
-    mono_nat_auth_own γT (1/2) T.
-
-  Definition ownTimeLocal T : iProp Σ :=
-    mono_nat_auth_own γT (1/2) T.
-
-  Definition ownTimeCptSnap T : iProp Σ :=
-    mono_nat_lb_own γT T.
-
-  Definition ownTimeSnap ts : iProp Σ :=
-     ownTimeCptSnap ts ∗ ownTimeStartsSnap ts.
-
-  Instance ownTimeSnap_Persistent :
-      ∀ i, Persistent (ownTimeSnap i).
+    Lemma ownSnapFragPersistent γt t k h :
+      Persistent (ownSnapFrag γt t k h).
     Proof. apply _. Qed.
 
-  (** ---------------- Propreties of global memory. ---------------- *)
+    (** Importantly, note that there is currently no relation between snapshots
+        for two given transactions. We only relate snapshots to the state of 
+        the global memory. *)
+    Definition ownSnapshotsAuth (Sγ : gmap nat gname) (S : snapshots) : iProp Σ :=
+      ownSnapshotsNamesAuth Sγ ∗
+      ([∗ map] t ↦ γt ; Mt ∈ Sγ ; S, ownTrnFrag t γt ∗ ownSnapAuthGname γt Mt).
 
-  Lemma ownMemSeen_lookup M k h :
-    ownMemMono M ⊢
-    ownMemSeen k h -∗
-    ∃ h', ⌜h `prefix_of` h' ∧ M !! k = Some h'⌝.
-  Proof.
-    iIntros "H1 H2".
-    iDestruct (own_valid_2 with "H1 H2")
-      as %[Hv1 Hv2]%auth_both_valid_discrete.
-    rewrite singleton_included_l in Hv1.
-    destruct Hv1 as (y & Hvy & Hv1).
-    rewrite Some_included_total in Hv1.
-    rewrite lookup_fmap in Hvy.
-    destruct (M !! k) eqn:Heq; rewrite Heq in Hvy;
-      simplify_eq /=; [| by inversion Hvy].
-    apply Some_equiv_inj in Hvy.
-    rewrite -Hvy to_max_prefix_list_included in Hv1.
-    destruct Hv1 as (l0 & Hl0).
-    fold_leibniz.
-    iPureIntro; exists l. split; last done.
-    by rewrite Hl0; apply prefix_app_r.
-  Qed.
+    Lemma ownSnapFrag_lookup Sγ S M γ t k h :
+      ownSnapshotsAuth Sγ S ⊢
+      ⌜Sγ !! t = Some γ⌝ -∗
+      ⌜S !! t = Some M⌝ -∗
+      ownSnapFrag γ t k h -∗
+      ∃ h', ⌜h `prefix_of` h' ∧ M !! k = Some h'⌝.
+    Proof.
+      iIntros "(HAuthNames & HAuth) %Hγ %HM #(Hf1 & Hf2)".
+      iDestruct (big_sepM2_lookup with "[$HAuth]") as "(_ & HauthM)"; try eauto.
+      iApply (ownSnapFragGname_lookup with "[$HauthM][$Hf2]").
+    Qed.
 
-  Lemma  ownMemSeen_Persistent k h :
-    Persistent (ownMemSeen k h).
-  Proof. apply _. Qed.
+    Lemma get_ownSnapFrag_prefix Sγ S M k h hl t γ:
+      Sγ !! t = Some γ →
+      S !! t = Some M →
+      M !! k = Some h →
+      hl `prefix_of` h →
+      ownSnapshotsAuth Sγ S ⊢
+      |==> ownSnapshotsAuth Sγ S ∗ ownSnapFrag γ t k hl.
+    Proof.
+      iIntros (Hsg HS HM Hpre) "(Htrs & Hauth)".
+      iDestruct (big_sepM2_lookup_acc with "[$Hauth]")
+        as "((#Ht & Ha) & Hacc)"; try eauto.
+      iMod (get_ownSnapFragGname_prefix γ M k h hl HM Hpre with "[Ha]")
+        as "(Ha & Hf)"; try eauto.
+      iFrame "#∗".
+      iApply "Hacc".
+      by iFrame "#∗".
+    Qed.
+    
+    Lemma get_ownSnapFrag Sγ S M t k h γ :
+      Sγ !! t = Some γ →
+      S !! t = Some M →
+      M !! k = Some h →
+      ownSnapshotsAuth Sγ S ⊢ |==>  ownSnapshotsAuth Sγ S ∗ ownSnapFrag γ t k h.
+    Proof.
+      iIntros (???) "Ha".
+      by iApply (get_ownSnapFrag_prefix with "[$Ha]").
+    Qed.
 
-(*  Seen_timeless k h :> Timeless (Seen k h); *)
+  End Snapshots.
 
-(* OwnMemKey_exclusive k h h' : *)
-(*         k ↦ₖ h ⊢ k ↦ₖ h' -∗ False; *)
+End Snapshot_Resources.
 
-(*     OwnLocalKey_exclusive k c v v' : *)
-(*         k ↦{c} v ⊢ k ↦{c} v' -∗ False; *)
+(*---------------------------------------------------------------------------*)
+(** ------------------- Resources for Global State ------------------------- *)
+(*---------------------------------------------------------------------------*)
+Section Global_Memory_Resources.
+  Context `{!anerisG Mdl Σ, !User_params, !IDBG Σ}.
 
+  (*---------------------------------------------------------------------------*)
+  (** ------------------- Monotone tracking of the memory -------------------- *)
+  (*---------------------------------------------------------------------------*)
+  Section MonotoneMemory.
+    Context (γGsnap : gname).
 
-  Lemma ownMemSeen_prefix k h h':
-    ownMemSeen k h ⊢ ownMemSeen k h' -∗
-    ⌜h `prefix_of` h' ∨ h' `prefix_of` h⌝.
-  Proof.
-    iIntros "Hobs1 Hobs2".
-    iDestruct (own_valid_2 with "Hobs1 Hobs2") as %Hvalid.
-    rewrite auth_frag_op_valid singleton_op singleton_valid
-      in Hvalid.
-    by rewrite to_max_prefix_list_op_valid_L in Hvalid.
-  Qed.
+    Definition ownMemSeen (k : Key) (h : list write_event) : iProp Σ :=
+      own γGsnap (◯ {[ k := to_max_prefix_list h]}).
+    
+    Definition ownMemMono (M : gmap Key (list write_event)) : iProp Σ :=
+      own γGsnap (● global_memUR M).
 
-  Lemma get_OwnMemSeen_prefix M k h hl:
+    Lemma ownMemSeen_lookup M k h :
+      ownMemMono M ⊢
+        ownMemSeen k h -∗
+        ∃ h', ⌜h `prefix_of` h' ∧ M !! k = Some h'⌝.
+    Proof.
+      iIntros "H1 H2".
+      iDestruct (own_valid_2 with "H1 H2")
+        as %[Hv1 Hv2]%auth_both_valid_discrete.
+      rewrite singleton_included_l in Hv1.
+      destruct Hv1 as (y & Hvy & Hv1).
+      rewrite Some_included_total in Hv1.
+      rewrite lookup_fmap in Hvy.
+      destruct (M !! k) eqn:Heq; rewrite Heq in Hvy;
+        simplify_eq /=; [| by inversion Hvy].
+      apply Some_equiv_inj in Hvy.
+      rewrite -Hvy to_max_prefix_list_included in Hv1.
+      destruct Hv1 as (l0 & Hl0).
+      fold_leibniz.
+      iPureIntro; exists l. split; last done.
+      by rewrite Hl0; apply prefix_app_r.
+    Qed.
+    Lemma ownMemSeen_Persistent k h :
+      Persistent (ownMemSeen k h).
+    Proof. apply _. Qed.
+    
+    Lemma ownMemSeen_prefix k h h':
+      ownMemSeen k h ⊢ ownMemSeen k h' -∗
+        ⌜h `prefix_of` h' ∨ h' `prefix_of` h⌝.
+    Proof.
+      iIntros "Hobs1 Hobs2".
+      iDestruct (own_valid_2 with "Hobs1 Hobs2") as %Hvalid.
+      rewrite auth_frag_op_valid singleton_op singleton_valid
+        in Hvalid.
+      by rewrite to_max_prefix_list_op_valid_L in Hvalid.
+    Qed.
+
+    Lemma get_OwnMemSeen_prefix M k h hl:
       M !! k = Some h →
       hl `prefix_of` h →
       ownMemMono M ⊢ |==> ownMemMono M ∗ ownMemSeen k hl.
-  Proof.
-    iIntros (HMk h_hl) "?".
-    iApply own_op.
-    iApply own_update; last done.
-    apply auth_update_dfrac_alloc.
-    {
-      apply gmap_core_id=>i x/lookup_singleton_Some[_<-].
-      apply max_prefix_list.mono_list_lb_core_id.
-    }
-    apply (@singleton_included_l _ _ _ (max_prefix_listR write_eventO)).
-    exists (to_max_prefix_list h).
-    split; first by rewrite lookup_fmap HMk.
-    apply Some_included_2.
-    apply (@to_max_prefix_list_included_L write_eventO); last done.
-    apply _.
-  Qed.
+    Proof.
+      iIntros (HMk h_hl) "?".
+      iApply own_op.
+      iApply own_update; last done.
+      apply auth_update_dfrac_alloc.
+      {
+        apply gmap_core_id=>i x/lookup_singleton_Some[_<-].
+        apply max_prefix_list.mono_list_lb_core_id.
+      }
+      apply (@singleton_included_l _ _ _ (max_prefix_listR write_eventO)).
+      exists (to_max_prefix_list h).
+      split; first by rewrite lookup_fmap HMk.
+      apply Some_included_2.
+      apply (@to_max_prefix_list_included_L write_eventO); last done.
+      apply _.
+    Qed.
 
-  Lemma get_OwnMemSeen M k h :
+    Lemma get_OwnMemSeen M k h :
       M !! k = Some h →
       ownMemMono M ⊢ |==> ownMemMono M ∗ ownMemSeen k h.
-  Proof.
-    intro HMk.
-    by iApply get_OwnMemSeen_prefix.
-  Qed.
+    Proof.
+      intro HMk.
+      by iApply get_OwnMemSeen_prefix.
+    Qed.
 
-  (** TODO: other needed lemmas. *)
+  End MonotoneMemory.
 
-End Resources.
+  (*---------------------------------------------------------------------------*)
+  (** ------------------- Monotone tracking of the memory -------------------- *)
+  (*---------------------------------------------------------------------------*)
+  Section GlobalMemory.
+    Context (γGauth γGsnap : gname).
+
+    Definition ownMemUser (k : Key) (h : (whist)) : iProp Σ :=
+      ghost_map_elem γGauth k (DfracOwn 1%Qp) h ∗ ownMemSeen γGsnap k h.
+
+    Definition ownMemAuthGlobal (M : global_mem) :=
+      ghost_map_auth γGauth (1/2)%Qp M.
+
+    Definition ownMemAuthLocal (M : global_mem) :=
+      ghost_map_auth γGauth (1/2)%Qp M.
+    
+    Definition ownMemGlobal (M : global_mem) : iProp Σ :=
+      ownMemAuthGlobal M ∗ ownMemMono γGsnap M.
+
+    (*  Seen_timeless k h :> Timeless (Seen k h); *)
+    (* OwnMemKey_exclusive k h h' : *)
+    (*         k ↦ₖ h ⊢ k ↦ₖ h' -∗ False; *)
+
+    (*     OwnLocalKey_exclusive k c v v' : *)
+    (*         k ↦{c} v ⊢ k ↦{c} v' -∗ False; *)
+    
+  End GlobalMemory.
+
+  (** ---------------- Time ---------------- *)
+  Section GlobalTime.
+    Context (γT : gname).
+    
+    Definition ownTimeGlobal T : iProp Σ :=
+      mono_nat_auth_own γT (1/2) T.
+
+    Definition ownTimeLocal T : iProp Σ :=
+      mono_nat_auth_own γT (1/2) T.
+
+    Definition ownTimeSnap T : iProp Σ :=
+      mono_nat_lb_own γT T.
+
+    Instance ownTimeSnap_Persistent :
+      ∀ i, Persistent (ownTimeSnap i).
+    Proof. apply _. Qed.
+
+   End GlobalTime.
+  
+End Global_Memory_Resources.
