aneris/examples/snapshot_isolation/proof/resources/local_invariant.v
@@ -11,30 +11,31 @@ From aneris.lib Require Import gen_heap_light.
 From aneris.aneris_lang.lib Require Import
      list_proof monitor_proof lock_proof map_proof.
 From aneris.aneris_lang.lib.serialization Require Import serialization_proof.
-From aneris.examples.snapshot_isolation.specs Require Import user_params.
-From aneris.examples.snapshot_isolation.proof Require Import
-     time events model.
+From aneris.examples.snapshot_isolation.proof Require Import model.
 From aneris.examples.snapshot_isolation.proof.resources Require Import
      resource_algebras server_resources.
 
 Section Local_Invariant.
 
   Context `{!anerisG Mdl Σ, !User_params, !IDBG Σ}.
-  Context (γGauth γT γTss : gname).
+  Context (γGauth γT γTrs : gname).
 
   Definition lkResDef (kvsL vnumL : loc) : iProp Σ :=
-    ∃ (kvsV : val) (T : Time) (Tss : gset nat)
-      (m : gmap Key val) (M : gmap Key (list write_event)),
+    ∃ (kvsV : val) (T : Time)
+      (m : gmap Key val) (Mc : global_mem) (S : snapshots)
+      (Sγ : gmap nat gname),
         ⌜is_map kvsV m⌝ ∗
-        ⌜kvsl_valid m M T Tss⌝ ∗
-        ⌜map_Forall (λ k l, Forall (λ we, KVS_Serializable (we_val we)) l) M⌝ ∗
-        ownMemAuthLocal γGauth M ∗
+        ⌜kvsl_valid m Mc S T⌝ ∗
+        ⌜map_Forall (λ k l, Forall (λ we, KVS_Serializable (we_val we)) l) Mc⌝ ∗
+        ownMemAuthLocal γGauth Mc ∗
         ownTimeLocal γT T ∗
-        ([∗ set] t ∈ Tss, ownTimeSnap γT γTss t) ∗
+        ([∗ map] t ↦γ;M ∈ Sγ;S, ownTrnFrag γTrs t γ ∗ ownSnapFragMemGname γ M) ∗
         kvsL ↦[ip_of_address KVS_address] kvsV ∗
         vnumL ↦[ip_of_address KVS_address] #T.
 
-  Definition server_lock_inv (γ : gname) (v : val) (kvsL vnumL : loc) : iProp Σ :=
-    is_lock (KVS_InvName .@ "lk") (ip_of_address KVS_address) γ v (lkResDef kvsL vnumL).
+  Definition server_lock_inv
+    (γlk : gname) (v : val) (kvsL vnumL : loc) : iProp Σ :=
+    is_lock (KVS_InvName .@ "lk") (ip_of_address KVS_address) γlk v
+      (lkResDef kvsL vnumL).
 
 End Local_Invariant.
