aneris/examples/snapshot_isolation/proof/utils.v
@@ -1,0 +1,35 @@
+From iris.algebra Require Import
+     agree auth excl gmap frac_auth excl_auth updates local_updates csum.
+From iris.algebra.lib Require Import mono_list.
+From iris.base_logic.lib Require Import mono_nat ghost_map.
+From iris.base_logic Require Import invariants.
+From iris.bi.lib Require Import fractional. 
+From iris.proofmode Require Import tactics.
+From aneris.prelude Require Import list.
+From aneris.algebra Require Import monotone.
+From aneris.aneris_lang Require Import lang resources resources inject.
+
+
+
+Lemma last_of_none_empty_list_is_some {A : Type} (l : list A) :
+    l ≠ [] → ∃ v, Some v = last (l).
+  Proof.
+    induction l.
+    1 : done.
+    destruct l; set_solver.
+  Qed.
+
+  Lemma last_in {A : Type} (l : list A) (a : A) :
+    last l  = Some a → In a l.
+  Proof.
+    intros Hyp.
+    induction l as [ | h l IH]; first inversion Hyp.
+    destruct l.
+    - inversion Hyp.
+      set_solver.
+    - inversion Hyp as [Hyp'].
+      apply IH in Hyp'.
+      set_solver.
+  Qed.
+
+  
